update

raindrops/Raindrops.fst
@@ -1,7 +1,6 @@
 module Raindrops
 
 open Bridge
-module LS = Lemmas.String
 
 (*
     If the number contains 3 as a factor, output 'Pling'.
@@ -9,18 +8,13 @@ module LS = Lemmas.String
     If the number contains 7 as a factor, output 'Plong'.
     If the number does not contain 3, 5, or 7 as a factor, just pass the number's digits straight through.
 *)
-val raindrop : native_int -> string
-let raindrop n = match of_int n with
-    | n when n % 3 <> 0 && n % 5 <> 0 && n % 7 <> 0 -> string_of_int n
-    | n -> (if n % 3 = 0 then "Pling" else "")
-            ^ (if n % 5 = 0 then "Plang" else "")
-            ^ (if n % 7 = 0 then "Plong" else "")
-
-val raindrop_cause_some_sound: (n:native_int) -> Lemma (raindrop n <> "")
-let raindrop_cause_some_sound n =
-    LS.empty_string_length_is_zero "";
-    match of_int n with
-    | n when n % 3 <> 0 && n % 5 <> 0 && n % 7 <> 0 -> ()
-    | n -> LS.not_empty_string_length_is_pos "Pling";
-            LS.not_empty_string_length_is_pos "Plang";
-            LS.not_empty_string_length_is_pos "Plong"
+val raindrop : (drop:native_int) -> Tot (sound:string{sound <> ""})
+let raindrop drop = match of_int drop with
+    | drop when drop % 3 <> 0 && drop % 5 <> 0 && drop % 7 <> 0 -> string_of_int drop
+    | drop -> (
+        let sound = (if drop % 3 = 0 then "Pling" else "")
+            ^ (if drop % 5 = 0 then "Plang" else "")
+            ^ (if drop % 7 = 0 then "Plong" else "") in
+        Lemmas.String.pos_length_string_is_not_empty sound;
+        sound
+    )
