Lemmas.String.fst
@@ -2,16 +2,20 @@ module Lemmas.String
 
 module S = FStar.String
 
-val string_of_int_return_not_empty_string: (n:int) -> Lemma (ensures S.length (string_of_int n) > 0 /\ (string_of_int n) <> "") [SMTPat (string_of_int n)]
+assume val string_of_int_return_not_empty_string: (n:int) -> Lemma (ensures string_of_int n <> "") [SMTPat (string_of_int n)]
 
-val strcat_add_length: (s1:string) -> (s2:string) -> Lemma (ensures (S.length s1) + (S.length s2) = (S.length (s1 ^ s2))) [SMTPat (s1 ^ s2)]
+assume val strcat_add_length: (s1:string) -> (s2:string) -> Lemma (ensures (S.length s1) + (S.length s2) = (S.length (s1 ^ s2))) [SMTPat (s1 ^ s2)]
 
-val string_length_is_nat: (s:string) -> Lemma (S.length s >= 0) [SMTPat (S.length s)]
+assume val strcat_empty_equal_1: (s:string) -> Lemma (ensures s ^ "" = s) [SMTPat (s ^ "")]
 
-val empty_string_length_is_zero: (s:string) -> Lemma (requires s = "") (ensures S.length s = 0)
+assume val strcat_empty_equal_2: (s:string) -> Lemma (ensures "" ^ s = s) [SMTPat ("" ^ s)]
 
-val zero_length_string_is_empty: (s:string) -> Lemma (requires S.length s = 0) (ensures s = "")
+assume val string_length_is_nat: (s:string) -> Lemma (S.length s >= 0) [SMTPat (S.length s)]
 
-val not_empty_string_length_is_pos: (s:string) -> Lemma (requires s <> "") (ensures S.length s > 0)
+assume val empty_string_length_is_zero: (s:string) -> Lemma (requires s = "") (ensures S.length s = 0)
 
-val pos_length_string_is_not_empty: (s:string) -> Lemma (requires S.length s > 0) (ensures s <> "")
+assume val zero_length_string_is_empty: (s:string) -> Lemma (requires S.length s = 0) (ensures s = "") [SMTPat (S.length s)]
+
+assume val not_empty_string_length_is_pos: (s:string) -> Lemma (requires s <> "") (ensures S.length s > 0)
+
+assume val pos_length_string_is_not_empty: (s:string) -> Lemma (requires S.length s > 0) (ensures s <> "") [SMTPat (S.length s)]
